wip rank -> num

tarjan_bigmin.v
@@ -13,7 +13,7 @@ Section tarjan.
 Variable (V : finType) (successors : V -> seq V).
 Notation edge := (grel successors).
 Notation gconnect := (connect edge).
-Notation infty := #|V|.
+Notation infty := #|V|.+1.
 
 (*************************************************)
 (* Connected components of the graph, abstractly *)
@@ -77,8 +77,8 @@ Definition split_after (T :eqType) (x : T) (s : seq T) :=
 Record env := Env {blacks : {set V}; stack : seq V; sccs : {set {set V}};
                    sn : nat; num: {ffun V -> nat}}.
 
-Definition set_infty (s : pred V) f := 
-  [ffun x => if x \in s then infty.+1 else f x].
+Definition set_infty (s : pred V) f :=
+  [ffun x => if s x then infty else f x].
 
 Definition add_stack x e :=
   Env (blacks e) (x :: stack e) (sccs e) (sn e).+1
@@ -90,18 +90,18 @@ Definition add_sccs x e :=
    Env (x |: blacks e) s3 ([set y in s2] |: sccs e)
        (sn e) (set_infty (mem s2) (num e)).
 
-Definition dfs1 (dfs' : {set V} -> env -> nat * env) (x : V) e :=
-    let: (m1, e1) := dfs' [set y in successors x] (add_stack x e) in
+Definition dfs1 (dfs : {set V} -> env -> nat * env) (x : V) e :=
+    let: (m1, e1) := dfs [set y in successors x] (add_stack x e) in
     if m1 >= sn e then (infty, add_sccs x e1) else (m1, add_blacks x e1).
 
-Definition dfs' dfs1 dfs' (roots : {set V}) e :=
+Definition dfs dfs1 dfs (roots : {set V}) e :=
   if [pick x in roots] isn't Some x then (infty, e)
   else let roots' := roots :\ x in
        let: (m1, e1) := if num e x != 0 then (num e x, e) else dfs1 x e in
-       let: (m2, e2) := dfs' roots' e1 in (minn m1 m2, e2).
+       let: (m2, e2) := dfs roots' e1 in (minn m1 m2, e2).
 
 Fixpoint tarjan_rec n : {set V} -> env -> nat * env :=
-  if n is n.+1 then dfs' (dfs1 (tarjan_rec n)) (tarjan_rec n)
+  if n is n.+1 then dfs (dfs1 (tarjan_rec n)) (tarjan_rec n)
   else fun r e => (infty, e).
 
 Let N := #|V| * #|V|.+1 + #|V|.
@@ -235,7 +235,7 @@ Inductive color4_spec x e : bool -> bool -> bool -> bool -> bool -> Type :=
 | Color4BlackStack of x \in blacks e & x \in stack e :
                         color4_spec x e true true false false false.
 
-Lemma colorP x e : wf_color e ->
+Lemma color4P x e : wf_color e ->
                    color4_spec x e (x \in blacks e) (x \in stack e)
                               (x \in cover (sccs e))
                               (x \in grays e) (x \in whites e).
@@ -251,39 +251,39 @@ Qed.
 
 Lemma stack_sccsF x e : wf_color e -> x \in stack e ->
   x \in cover (sccs e) = false.
-Proof. by case/colorP. Qed.
+Proof. by case/color4P. Qed.
 
 Lemma grays_blacksF x e : wf_color e -> x \in grays e ->
    x \in blacks e = false.
-Proof. by case/colorP. Qed.
+Proof. by case/color4P. Qed.
 
 Lemma grays_sccsF x e : wf_color e -> x \in grays e ->
    x \in cover (sccs e) = false.
-Proof. by case/colorP. Qed.
+Proof. by case/color4P. Qed.
 
 Lemma sccs_stackF x e : wf_color e ->
   x \in cover (sccs e) -> x \in stack e = false.
-Proof. by case/colorP. Qed.
+Proof. by case/color4P. Qed.
 
 Lemma sccs_blacks x e : wf_color e -> x \in cover (sccs e) -> x \in blacks e.
-Proof. by case/colorP. Qed.
+Proof. by case/color4P. Qed.
 
-Lemma add_stack_ewf x e : x \in whites e -> wf_color e -> wf_color (add_stack x e).
+Lemma add_stack_cwf x e : x \in whites e -> wf_color e -> wf_color (add_stack x e).
 Proof.
 move=> x_white e_wf; split=> /=; do ?
   by [exact: wf_sccs|rewrite whites_stackF ?wf_uniq].
 move=> y; rewrite grays_add_stack // !inE.
-by case: (_ == _) colorP => [] [].
+by case: (_ == _) color4P => [] [].
 Qed.
 
-Lemma add_blacks_ewf x e : x \in grays e -> wf_color e -> wf_color (add_blacks x e).
+Lemma add_blacks_cwf x e : x \in grays e -> wf_color e -> wf_color (add_blacks x e).
 Proof.
 move=> x_gray e_wf; split => //=; last 2 first.
 - by rewrite subsetU // wf_sccs // orbT.
 - exact: wf_uniq.
 move=> y; rewrite grays_add_blacks !inE.
-have [->|] := altP (y =P x); case: colorP => //.
-by case: colorP x_gray.
+have [->|] := altP (y =P x); case: color4P => //.
+by case: color4P x_gray.
 Qed.
 
 Lemma add_sccs_wf x e :
@@ -304,155 +304,109 @@ have [->|neq_xy] //= := altP (y =P x); rewrite ?(andbT, andbF).
   case: splitP new_blacks s_uniq => //=; first by rewrite grays_stack.
   move=> s1 s2 s1x_blacks s_uniq; rewrite grays_sccsF // andbT.
   by rewrite (uniq_catRL s_uniq) // mem_cat mem_rcons mem_head.
-case: colorP; rewrite ?(andbT, andbF, orbT, orbF) //=.
-  by move=> y_sccs; apply: contraTF y_sccs => /mem_drop; case: colorP.
+case: color4P; rewrite ?(andbT, andbF, orbT, orbF) //=.
+  by move=> y_sccs; apply: contraTF y_sccs => /mem_drop; case: color4P.
 move=> y_blacks; case: splitP s_uniq; first by rewrite grays_stack.
 by move=> s1 s2 s_uniq y_in; apply: uniq_catRL.
 Qed.
+
+Inductive stack_spec x e : bool -> bool -> bool -> bool -> bool -> Type :=
+| StackWhite of x \in whites e : stack_spec x e true false false false false
+| StackStack of x \in stack e :
+                       stack_spec x e false true false (x \in grays e) (x \in blacks e)
+| StackSccs  of x \in cover (sccs e) :
+                        stack_spec x e false false true false true.
+
+Lemma stackP x e : wf_color e ->
+  stack_spec x e (x \in whites e) (x \in stack e) (x \in cover (sccs e))
+                              (x \in grays e) (x \in blacks e).
+Proof.
+move=> e_cwf; set xb := x \in blacks _; set xg := x \in grays e.
+case: color4P => //.
+- by move=> /grays_stack; constructor.
+- by rewrite /xg /xb; case: color4P => //; constructor.
+- by rewrite /xg /xb; case: color4P => //; constructor.
+- by constructor.
+Qed.
+
+Lemma set_infty_eq0 (P : pred V) f x : (forall x, P x -> f x != 0) ->
+  (set_infty P f x == 0) = (f x == 0).
+Proof.
+Admitted.
+
+Lemma set_infty_eq_infty (P : pred V) f x :
+  (set_infty P f x == infty) = P x || (f x == infty).
+Proof.
+Admitted.
+
+Lemma set_infty_infty (P : pred V) f x : P x -> set_infty P f x = infty.
+Proof. by rewrite /set_infty ffunE/=; case: (P _). Qed.
+
+Lemma set_infty_id (P : pred V) f x : ~~ P x -> set_infty P f x = f x.
+Proof. by rewrite /set_infty ffunE/=; case: (P _). Qed.
+
 
 (*******************)
 (* Well formed env *)
 (*******************)
 
+Notation precedes x y e := (index x (stack e) <= index y (stack e)).
+Local Notation "x '<[' e ']=' y" := (precedes x y e)
+  (at level 10, format "x  '<[' e ]=  y").
+
 Record wf_num e := WfNum {
    wf_num0      : forall x, (num e x == 0) = (x \in whites e);
-   wf_num_infty : forall x, (num e x == infty.+1) = (x \in cover (sccs e));
-   wf_num_le    : forall x, num e x < sn e;
-   wf_sn        : sn e = #|grays e :|: blacks e|;
-   wf_num_stack : {in stack e &, forall x y, 
-                       (num e x <= num e y) = (index y (stack e) <= index x (stack e))}
+   wf_num_infty : forall x, (num e x == infty) = (x \in cover (sccs e));
+   wf_num_lt    : forall x, num e x != infty -> num e x < sn e;
+   wf_sn        : sn e = #|grays e :|: blacks e|.+1;
+   wf_num_stack : {in stack e &, forall x y,  (num e x <= num e y) = (y <[e]= x)}
 }.
 
-(* Lemma add_stack_nwf x e : x \in whites e -> wf_color e -> wf_num e -> wf_num (add_stack x e). *)
-(* Proof. *)
-(* move=> x_whites e_nwf; split=> //= [y|y|y||]. *)
-(*   rewrite !ffunE/=. *)
+Lemma ord_num x e : wf_num e -> @inord infty (num e x) = num e x :> nat.
+Admitted.
 
+Lemma add_stack_nwf x e : x \in whites e -> wf_color e ->
+  wf_num e -> wf_num (add_stack x e).
+Proof.
+Admitted.
 
+ Lemma add_blacks_nwf x e : x \in grays e -> wf_color e ->
+   wf_num e -> wf_num (add_blacks x e).
+Admitted.
 
- 
-(* move=> x_white e_wf; split=> /=; do ? *)
-(*   by [exact: wf_sccs|rewrite whites_stackF ?wf_uniq]. *)
-(* move=> y; rewrite grays_add_stack // !inE. *)
-(* by case: (_ == _) colorP => [] []. *)
-(* Qed. *)
+ Lemma add_sccs_nwf x e :
+   take (index x (stack e)) (stack e) \subset blacks e ->
+   x \in grays e -> wf_color e ->
+   wf_num e -> wf_num (add_stack x e).
+Admitted.
 
-(* Lemma add_blacks_ewf x e : x \in grays e -> wf_color e -> wf_color (add_blacks x e). *)
-(* Proof. *)
-(* move=> x_gray e_wf; split => //=; last 2 first. *)
-(* - by rewrite subsetU // wf_sccs // orbT. *)
-(* - exact: wf_uniq. *)
-(* move=> y; rewrite grays_add_blacks !inE. *)
-(* have [->|] := altP (y =P x); case: colorP => //. *)
-(* by case: colorP x_gray. *)
-(* Qed. *)
+Lemma num_inftyP e x : reflect (num e x = infty) (x \in cover (sccs e)).
+Proof. Admitted.
 
+Lemma sn_small e : wf_num e -> sn e <= infty.
+Proof. by move=> e_nwf; rewrite wf_sn// ltnS max_card. Qed.
 
-(* Lemma add_sccs_wf x e : *)
-(*   take (index x (stack e)) (stack e) \subset blacks e -> *)
-(*   x \in grays e -> wf_color e -> wf_color (add_sccs x e). *)
-(* Proof. *)
-(* move=> new_blacks x_gray e_wf. *)
-(* have [s_def /subsetP sccs_blacks s_uniq] := e_wf. *)
-(* split => //=; last first. *)
-(* - by rewrite (subseq_uniq (drop_subseq _ _)). *)
-(* - apply/subsetP=> y; rewrite !inE. *)
-(*   rewrite /cover bigcup_setU inE big_set1 !inE /= => /orP[|/sccs_blacks->]; *)
-(*     last by rewrite !orbT. *)
-(*   by rewrite mem_rcons !inE; case: eqP => //= _ /(subsetP new_blacks). *)
-(* move=> y; rewrite !inE /cover bigcup_setU inE big_set1 !inE !negb_or. *)
-(* rewrite graysE ?inE //. *)
-(* have [->|neq_xy] //= := altP (y =P x); rewrite ?(andbT, andbF). *)
-(*   case: splitP new_blacks s_uniq => //=; first by rewrite grays_stack. *)
-(*   move=> s1 s2 s1x_blacks s_uniq; rewrite grays_sccsF // andbT. *)
-(*   by rewrite (uniq_catRL s_uniq) // mem_cat mem_rcons mem_head. *)
-(* case: colorP; rewrite ?(andbT, andbF, orbT, orbF) //=. *)
-(*   by move=> y_sccs; apply: contraTF y_sccs => /mem_drop; case: colorP. *)
-(* move=> y_blacks; case: splitP s_uniq; first by rewrite grays_stack. *)
-(* by move=> s1 s2 s_uniq y_in; apply: uniq_catRL. *)
-(* Qed. *)
+Lemma num_stackP e x : wf_color e -> wf_num e ->
+   (x \in stack e) = (0 < num e x < sn e).
+Proof.
+move=> e_cwf e_nwf; symmetry; rewrite lt0n wf_num0//; case: stackP => //=.
+  by move=> x_stack; rewrite wf_num_lt // wf_num_infty//; case: stackP x_stack.
+by rewrite -wf_num_infty => // /eqP->; rewrite ltnNge sn_small.
+Qed.
 
-
-(***************)
-(* Rank Theory *)
-(***************)
-
-(* Lemma rankE x stack : *)
-(*   rank x stack = if x \in stack then index x (rev stack) else infty. *)
-(* Proof. *)
-(* elim: stack => [|a s /= ->] //. *)
-(* have [->|neq_xa] /= := altP eqP; rewrite rev_cons -cats1. *)
-(*   by rewrite mem_head index_cat mem_rev /= eqxx addn0 size_rev; case: in_mem. *)
-(* by rewrite in_cons (negPf neq_xa) /= index_cat /= mem_rev; case: in_mem. *)
-(* Qed. *)
-
-(* Lemma rank_cons x y s : rank x (y :: s) = *)
-(*   if (x == y) && (x \notin s) then size s else rank x s. *)
-(* Proof. by []. Qed. *)
-
-(* Lemma rank_catl x s s' : x \in s' -> rank x (s ++ s') = rank x s'. *)
-(* Proof. *)
-(* by move=> x_s; rewrite !rankE rev_cat mem_cat x_s orbT index_cat mem_rev x_s. *)
-(* Qed. *)
-
-(* Lemma rank_catr x s s' : *)
-(*   x \in s -> x \notin s' -> rank x (s ++ s') = size s' + rank x s. *)
-(* Proof. *)
-(* move=> x_s xNs'; rewrite !rankE rev_cat mem_cat x_s /=. *)
-(* by rewrite index_cat mem_rev (negPf xNs') size_rev. *)
-(* Qed. *)
-
-(* Lemma rank_small x s : uniq s -> (rank x s < size s) = (x \in s). *)
-(* Proof. *)
-(* move=> s_uniq; rewrite rankE; case: (boolP (x \in s)) => [xNs|_]. *)
-(*   by rewrite -size_rev index_mem mem_rev. *)
-(* apply: negbTE; rewrite -ltnNge ltnS cardE uniq_leq_size //. *)
-(* by move=> y; rewrite mem_enum. *)
-(* Qed. *)
-
-(* Arguments rank : simpl never. *)
-
-(* Lemma rank_le x (s : seq V) : uniq s -> rank x s <= infty. *)
-(* Proof. *)
-(* move=> s_uniq; rewrite rankE; case: ifP => // x_s. *)
-(* by rewrite (leq_trans (index_size _ _)) ?size_rev -?(card_uniqP _) // max_card. *)
-(* Qed. *)
-
-(* Lemma rank_lt x (s : seq V) : uniq s -> (rank x s < infty) = (x \in s). *)
-(* Proof. *)
-(* rewrite rankE; case: ifPn; rewrite ?ltnn // => x_s s_uniq. *)
-(* rewrite (@leq_trans (size (rev s))) ?index_mem ?mem_rev ?size_rev //. *)
-(* by rewrite -?(card_uniqP _) // max_card. *)
-(* Qed. *)
-
-(* Lemma rank_infty x (s : seq V) : x \notin s -> rank x s = infty. *)
-(* Proof. by rewrite rankE => /negPf->. Qed. *)
-
-(* Lemma rank_mem x s : x \in s -> rank x s < size s. *)
-(* Proof. by move=> x_s; rewrite rankE x_s -size_rev index_mem mem_rev. Qed. *)
-
-(* Lemma rank_le_head s z x : x \notin s -> z \in s -> *)
-(*   rank z (x :: s) < rank x (x :: s). *)
-(* Proof. *)
-(* by move=> xNs z_s; rewrite !rank_cons z_s andbF eqxx xNs /= rank_mem. *)
-(* Qed. *)
-
-(* Lemma ord_rank x s : uniq s -> @inord #|V| (rank x s) = rank x s :> nat. *)
-(* Proof. by move=> s_uniq; rewrite inordK // ltnS rank_le. Qed. *)
-
-(********************)
-(*   Main Proof !   *)
-(********************)
+Lemma stack_neq_infty e x : wf_color e -> wf_num e ->
+   x \in stack e -> (num e) x != infty.
+Proof. by move=> e_cwf e_nwf x_stack; rewrite wf_num_infty// stack_sccsF. Qed.
 
 Definition noblack_to_white e :=
   forall x, x \in blacks e -> [disjoint successors x & whites e].
 
 Inductive wf_graph e := WfGraph {
   wf_grays_to_stack : {in grays e & stack e, forall x y,
-         (rank x (stack e) <= rank y (stack e)) -> gconnect x y};
+         (num e x <= num e y) -> gconnect x y};
   wf_stack_to_grays : forall y, y \in stack e ->
                       exists x, [/\ x \in grays e,
-     (rank x (stack e) <= rank y (stack e)) & gconnect y x]
+     (num e x <= num e y) & gconnect y x]
   }.
 
 Definition access_to e (roots : {set V}) :=
@@ -461,10 +415,11 @@ Definition access_to e (roots : {set V}) :=
 Definition black_gsccs e := [set scc in gsccs | scc \subset blacks e].
 
 Record invariants (e : env) := Invariants {
-  pre_wf_color : wf_color e;
-  pre_wf_graph : wf_graph e;
+  inv_wf_color : wf_color e;
+  inv_wf_num   : wf_num e;
+  inv_wf_graph : wf_graph e;
   wf_noblack_towhite : noblack_to_white e;
-  pre_sccs : sccs e = black_gsccs e;
+  inv_sccs : sccs e = black_gsccs e;
 }.
 
 Record pre_dfs (roots : {set V}) (e : env) := PreDfs {
@@ -473,24 +428,22 @@ Record pre_dfs (roots : {set V}) (e : env) := PreDfs {
 }.
 
 Lemma add_stack_gwf e w :
-  access_to e [set w] -> wf_color e -> w \in whites e -> wf_graph e ->
+  access_to e [set w] -> wf_color e -> wf_num e -> w \in whites e -> wf_graph e ->
   wf_graph (add_stack w e).
 Proof.
-move=> grays_to e_wf w_white [gs sg]; split.
-  rewrite grays_add_stack //= => x y; rewrite rank_cons !inE.
-  move=> /orP[/eqP->|xg] /orP[/eqP->|/=ys];
-  rewrite ?rank_cons ?eqxx ?(@whites_stackF w) ?xs ?ys ?(andbF, andbT) //=.
-  + by rewrite leqNgt rank_small ?wf_uniq // ys.
-  + by move=> _; rewrite grays_to ?inE.
-  + by rewrite grays_stack // andbF; apply: gs.
+move=> grays_to e_cwf e_nwf w_white [gs sg]; split.
+  rewrite grays_add_stack //= => x y. rewrite !ffunE !inE /=.
+  have [-> _|neq_xw /= x_gray] := altP eqP;
+  have [-> _|neq_yw /= y_stack]// := altP eqP.
+  - by rewrite leqNgt wf_num_lt// stack_neq_infty.
+  - by move=> _; rewrite grays_to ?inE.
+  - exact: gs.
 move=> y; rewrite inE => /predU1P [->|].
   by exists w; rewrite ?grays_add_stack ?inE ?eqxx.
 move=> y_stack; have /sg [x [x_gray le_xy y_to_x]] := y_stack.
-exists x; split=> //.
-  by rewrite grays_add_stack // inE x_gray orbT.
-rewrite stack_add_stack !rank_cons [x == w]negbTE /= 1?[y == w]negbTE //=.
-  by apply: contraTneq y_stack => ->; rewrite whites_stackF.
-by apply: contraTneq x_gray => ->; rewrite whites_graysF.
+exists x; split=> //; first by rewrite grays_add_stack // inE x_gray orbT.
+rewrite /= !ffunE/= !ifN//; apply: contraTneq w_white => <-;
+by case: color4P y_stack x_gray.
 Qed.
 
 Lemma add_stack_pre e w :
@@ -531,8 +484,9 @@ Qed.
 Definition subenv e1 e2 :=
   [&&  grays e1 == grays e2,
        blacks e1 \subset blacks e2,
-       sccs e1 \subset sccs e2 &
-       [exists n : 'I_infty.+1, stack e1 == drop n (stack e2)]].
+       sccs e1 \subset sccs e2,
+       [forall x in stack e1, num e2 x == num e1 x] &
+       [exists n : 'I_infty, stack e1 == drop n (stack e2)]].
 
 Lemma subenv_grays e1 e2 : subenv e1 e2 -> grays e2 = grays e1.
 Proof. by move=> /and4P [/eqP]. Qed.
@@ -543,9 +497,16 @@ Proof. by move=> /and4P []. Qed.
 Lemma subenv_sccs e1 e2 : subenv e1 e2 -> sccs e1 \subset sccs e2.
 Proof. by move=> /and4P []. Qed.
 
+Lemma subenv_num e1 e2 : subenv e1 e2 ->
+  {in stack e1, forall x, num e2 x = num e1 x}.
+Admitted.
+
+Lemma subenv_sn e1 e2 : subenv e1 e2 -> sn e1 <= sn e2.
+Admitted.
+
 Lemma subenvN_subproof e1 e2 : subenv e1 e2 ->
   {n : nat | stack e1 = drop n (stack e2)}.
-Proof. by move=> /and4P [_ _ _ /existsP /sigW[n /eqP]]; exists n. Qed.
+Proof. by move=> /and5P [_ _ _ _ /existsP /sigW[n /eqP]]; exists n. Qed.
 
 Definition subenvN e1 e2 :=
   if subenv e1 e2 =P true isn't ReflectT e12 then 0
@@ -559,7 +520,7 @@ Lemma subenv_take e1 e2 : wf_color e2 -> subenv e1 e2 ->
   take (subenvN e1 e2) (stack e2) \subset blacks e2.
 Proof.
 set n := subenvN e1 e2; move=> e2_wf e12; apply/subsetP=> x x_p2.
-suff: (x \in stack e2) && (x \notin grays e2) by case: colorP.
+suff: (x \in stack e2) && (x \notin grays e2) by case: color4P.
 rewrite (mem_take x_p2) (subenv_grays e12) /=.
 apply: contraTN isT => /grays_stack.
 have := wf_uniq e2_wf; rewrite -[stack e2](cat_take_drop n) => s12_uniq.
@@ -568,7 +529,7 @@ Qed.
 
 Lemma uniq_ex_drop (s1 s2 : seq V) :
    uniq s2 -> (exists s, s2 = s ++ s1) ->
-   exists n : 'I_infty.+1, s1 = drop n s2.
+   exists n : 'I_infty, s1 = drop n s2.
 Proof.
 move=> s2_uniq [s s2_def]; exists (inord (size s)).
 rewrite s2_def inordK ?drop_cat ?ltnn ?subnn ?drop0 // ltnS.
@@ -595,14 +556,15 @@ Proof.
 move=> e2_wf e12; rewrite whitesE -(subenv_grays e12) setDE setCK setIC -setDE.
 rewrite setDUl setDE setCU setIA setICr set0I set0U.
 rewrite setDUr (setIidPr _) // [_ :\: grays _](setDidPl _) ?subsetDl //.
-by apply/pred0P => y /=; case: colorP.
+by apply/pred0P => y /=; case: color4P.
 Qed.
 
 Lemma subenv_refl : reflexive subenv.
 Proof.
 move=> e; rewrite /subenv eqxx !subxx /=.
-by apply/existsP; exists ord0; rewrite drop0.
-Qed.
+(* by apply/existsP; exists ord0; rewrite drop0. *)
+(* Qed. *)
+Admitted.
 Hint Resolve subenv_refl.
 
 Lemma subenvee e : subenv e e. Proof. exact: subenv_refl. Qed.
@@ -615,26 +577,59 @@ move=> e2_wf e3_wf e12 e23; rewrite /subenv.
 rewrite (subenv_grays e23) (subenv_grays e12) eqxx.
 rewrite (subset_trans (subenv_blacks e12)) ?subenv_blacks //.
 rewrite (subset_trans (subenv_sccs e12)) ?subenv_sccs //=.
+apply/andP; split; first admit.
 apply/'exists_eqP; apply: uniq_ex_drop; first exact: wf_uniq.
 case: (subenv_stackP _ e23) => // s2 -> _.
 case: (subenv_stackP _ e12) => // s1 -> _.
 by exists (s2 ++ s1); rewrite catA.
+(* Qed. *)
+Admitted.
+
+Lemma subenv_gray_le e1 e2 x y : subenv (add_stack x e1) e2 ->
+   wf_color e2 -> wf_num e2 -> y \in grays e2 -> num e2 y <= num e2 x.
+Proof.
+move=> subxe12 e2_cwf e2_nwf y_gray.
+case: (@subenv_stackP (add_stack x e1) e2) => // s s_def sb.
+rewrite wf_num_stack //; last 2 first.
+- by case: color4P y_gray.
+- by rewrite s_def mem_cat /= mem_head orbT.
+rewrite s_def !index_cat.
+rewrite !ifN /=; first by rewrite leq_add2l eqxx; case: ifPn => //=.
+   by apply: contraTN y_gray => /(subsetP sb); case: color4P.
+have := wf_uniq e2_cwf; rewrite s_def => /(@uniq_catRL _ x).
+by rewrite mem_cat mem_head orbT -s_def wf_uniq// => <-.
+Qed.
+
+Lemma subenv_stack_gt e1 e2 x y : subenv e1 e2 ->
+   wf_num e1 -> wf_color e1 -> wf_color e2 -> wf_num e2 -> x \in stack e1 ->
+   y \in stack e2 -> y \notin stack e1 -> num e2 x < num e2 y.
+Proof.
+move=> sube12 e1_nwf e1_cwf e2_cwf e2_nwf x_stack1 y_stack2 yNstack1.
+case: (@subenv_stackP e1 e2) => // s s_def _.
+rewrite ltnNge wf_num_stack //; last first.
+  by rewrite s_def mem_cat x_stack1 orbT.
+rewrite s_def !index_cat; have ys : y \in s.
+  by have := y_stack2; rewrite s_def mem_cat (negPf yNstack1) orbF.
+rewrite ifN; last first.
+  have := wf_uniq e2_cwf; rewrite s_def => /(@uniq_catRL _ x).
+  by rewrite mem_cat x_stack1 orbT -s_def wf_uniq// => <-.
+by rewrite ifT// -ltnNge (@leq_trans (size s))// ?index_mem// leq_addr.
 Qed.
 
 Record post_dfs (roots : {set V}) (e e' : env) (m : nat) := PostDfs {
   post_invariants : invariants e';
   post_subenv : subenv e e';
   post_whites : whites e' = whites e :\: \bigcup_(x in roots) wreach e x;
-  post_rank : m = \min_(y in \bigcup_(x in roots) wreach e x)
-                @inord #|V| (rank y (stack e'));
+  post_num : m = \min_(y in \bigcup_(x in roots) wreach e x)
+                      @inord infty (num e' y);
 }.
 
 Definition dfs1_correct (dfs1 : V -> env -> nat * env) x e :=
   (x \in whites e) -> pre_dfs [set x] e ->
   let (m, e') := dfs1 x e in post_dfs [set x] e e' m.
 
-Definition dfs'_correct (dfs' : {set V} -> env -> nat * env) roots e :=
-  pre_dfs roots e -> let (m, e') := dfs' roots e in post_dfs roots e e' m.
+Definition dfs_correct (dfs : {set V} -> env -> nat * env) roots e :=
+  pre_dfs roots e -> let (m, e') := dfs roots e in post_dfs roots e e' m.
 
 Lemma pre_dfs_subroots (roots roots' : {set V}) e : roots' \subset roots ->
   pre_dfs roots e -> pre_dfs roots' e.
@@ -643,56 +638,57 @@ move=> sub_roots [to_roots [e_wf e_gwf black_sccs Nbw]]; split=> //.
 by move=> x x_gray y y_roots'; rewrite to_roots //; apply: subsetP y_roots'.
 Qed.
 
-Lemma dfs'_is_correct dfs1 dfsrec' (roots : {set V}) e :
+Lemma subND1 (T : finType) (A : {set T}) (x : T) : x \notin A -> A :\ x = A.
+Proof. by move=> xNA; rewrite (setDidPl _) ?disjoints1. Qed.
+
+Lemma dfs_is_correct dfs1 dfsrec (roots : {set V}) e :
   (forall x, x \in roots -> dfs1_correct dfs1 x e) ->
   (forall x, x \in roots -> forall e1, whites e1 \subset whites e ->
-         dfs'_correct dfsrec' (roots :\ x) e1) ->
-  dfs'_correct (dfs' dfs1 dfsrec') roots e.
+         dfs_correct dfsrec (roots :\ x) e1) ->
+  dfs_correct (dfs dfs1 dfsrec) roots e.
 Proof.
-move=> dfs1_is_correct dfs'_is_correct; rewrite /dfs'_correct /dfs'.
+move=> dfs1_is_correct dfs_is_correct; rewrite /dfs_correct /dfs.
 case: pickP => [x|no_roots]; last first.
   have roots0 : roots = set0 by apply/setP=> y; rewrite no_roots inE.
   move=> [gto_roots [e_wf e_gwf black_sccs]].
-  by split=> //; rewrite ?roots0 ?big_set0 ?setD0.
-move=> x_root; have := dfs'_is_correct _ x_root; rewrite /dfs'_correct.
-move=> dfsrec'_correct pre.
+  by split; rewrite ?roots0 ?big_set0 ?setD0.
+move=> x_root; have := dfs_is_correct _ x_root; rewrite /dfs_correct.
+move=> dfsrec_correct pre.
 have [to_roots [e_wf e_gwf Nbw black_sccs]] := pre.
 have e_uniq := @wf_uniq _ e_wf.
-case: ifPn=> [xsVb|xNsVb].
-  move: dfsrec'_correct => /(_ _ (subxx _)); case: (dfsrec' _ _) => [m2 e1].
+rewrite wf_num0 //; have [xw|xNw]/= := boolP (x \in _); last first.
+  move: dfsrec_correct => /(_ _ (subxx _)).
+  case: (dfsrec _ _) => [m2 e1].
   case; first exact: (pre_dfs_subroots (subD1set _ _)).
-  move=> [e1_wf e1_gwf Nbw1 sccs_e1] sube1 whites1 m2_min.
+  move=> [e1_wf e1_nwf e1_gwf Nbw1 sccs_e1] sube1 whites1 m2_min.
   have [//|s1 s1_def sb] := subenv_stackP _ sube1.
   have e1_uniq := wf_uniq e1_wf.
   split=> //.
     rewrite -(setD1K x_root) big_setU1 ?setD11 //=.
-    rewrite -setDDl whites1 Nwreach; last by case: colorP xsVb.
-    by rewrite [whites e :\ _](setDidPl _) // disjoints1; case: colorP xsVb.
+    by rewrite -setDDl whites1 Nwreach ?(subND1 xNw).
   rewrite -(setD1K x_root) big_setU1 ?setD11 // bigmin_setU /= m2_min.
-  congr (minn _ _); rewrite Nwreach; last by case: colorP xsVb.
-  rewrite big_set1 ord_rank // s1_def.
-  case: (boolP (_ \in stack e)) xsVb => /= [/rank_catl->|xNs x_black] //.
-  rewrite !rank_infty // -s1_def; case: colorP xNs x_black => //.
-  by move=> /(subsetP (subset_cover (subenv_sccs sube1))); case: colorP.
+  congr (minn _ _); rewrite Nwreach // big_set1 ord_num //.
+  case: stackP xNw => // [x_stack|x_sccs] _; first exact/esym/subenv_num.
+    rewrite ?(num_inftyP _ _ _) //.
+    by apply: (subsetP (subset_cover (subenv_sccs _))) x_sccs.
 have := dfs1_is_correct _ x_root; rewrite /dfs1_correct.
 case: (dfs1 _ _) => [m1 e1] post_dfs1.
-move: dfsrec'_correct => /(_ e1).
-case: (dfsrec' _ _) => [m2 e2] post_dfs' {dfs1_is_correct dfs'_is_correct}.
-have x_white : x \in whites e by case: colorP xNsVb.
-have := post_dfs1 x_white (pre_dfs_subroots _ pre).
+move: dfsrec_correct => /(_ e1).
+case: (dfsrec _ _) => [m2 e2] post_dfs {dfs1_is_correct dfs_is_correct}.
+have := post_dfs1 xw (pre_dfs_subroots _ pre).
 rewrite sub1set x_root => /(_ isT) {post_dfs1}.
-case=> [[e1_wf e1_gwf Nbw1 sccs_e1] sube1 whites1 m1_min].
+case=> [[e1_wf e1_cwf e1_gwf Nbw1 sccs_e1] sube1 whites1 m1_min].
 have [//|s1 s1_def s1b] := subenv_stackP _ sube1.
 have e1_uniq := wf_uniq e1_wf.
 rewrite big_set1 in whites1 m1_min.
-case: post_dfs'.
+case: post_dfs.
 - by rewrite subenv_whites.
 - split=> // y z; rewrite graysE !inE s1_def mem_cat.
   case: (y \in s1) (subsetP s1b y) => //= [->//|_ /andP[yNb ys]].
   move=> /andP[_ z_roots]; rewrite to_roots // graysE !inE.
   rewrite ys andbT; apply: contraNN yNb; apply/subsetP.
   by rewrite subenv_blacks.
-move=> [e2_wf e2_gwf Nbw2 sccs_e2] sube2 whites2 m2_min.
+move=> [e2_wf e2_cwf e2_gwf Nbw2 sccs_e2] sube2 whites2 m2_min.
 have [//|s2 s2_def s2b] := subenv_stackP _ sube2.
 have e2_uniq := wf_uniq e2_wf.
 have split_wreach : \bigcup_(y in roots) wreach e y =
@@ -712,33 +708,33 @@ split => //; first exact: subenv_trans sube2.
   by rewrite whites2 whites1 split_wreach setDDl.
 rewrite m1_min m2_min split_wreach bigmin_setU /=.
 congr (minn (val _) _); apply: eq_bigr => y xy; apply/val_inj=> /=.
-rewrite !ord_rank //.
+rewrite !ord_num //.
 have /orP[ys|ysccs] : (y \in stack e1) || (y \in cover (sccs e1)).
-+ suff: y \notin whites e1 by case: colorP.
++ suff: y \notin whites e1 by case: color4P.
   by rewrite whites1 inE xy.
-+ by rewrite s2_def rank_catl.
-+ rewrite !rank_infty ?sccs_stackF //.
-  by apply: subsetP ysccs; rewrite subset_cover ?subenv_sccs.
++ exact/esym/subenv_num.
+rewrite ?(num_inftyP _ _ _) //.
+by apply: (subsetP (subset_cover (subenv_sccs _))) ysccs.
 Qed.
 
-Lemma dfs1_is_correct dfs' (x : V) e :
-  (dfs'_correct dfs' [set y | edge x y] (add_stack x e)) ->
-  dfs1_correct (dfs1 dfs') x e.
+Lemma dfs1_is_correct dfs (x : V) e :
+  (dfs_correct dfs [set y | edge x y] (add_stack x e)) ->
+  dfs1_correct (dfs1 dfs) x e.
 Proof.
-rewrite /dfs1 /dfs1_correct /dfs'_correct; case: (dfs' _ _) => m1 e1.
-move=> post_dfs'; set m := rank x _.
-move=> x_white [access_to_x [e_wf e_gwf Nbw black_sccs]].
+rewrite /dfs1 /dfs1_correct /dfs_correct; case: (dfs _ _) => m1 e1.
+move=> post_dfs; set m := sn e.
+move=> x_white [access_to_x [e_wf e_cwf e_gwf Nbw black_sccs]].
 have e_uniq := @wf_uniq _ e_wf.
-case: post_dfs' => //=.
+case: post_dfs => //=.
   split => //.
     move=> y z; rewrite grays_add_stack // => /setU1P [->|y_gray];
     rewrite inE => /(@connect1 _ edge) //.
     by apply/connect_trans/access_to_x; rewrite ?set11.
-  split=> //; do?[exact: add_stack_ewf|exact: add_stack_gwf].
+    split=> //; do?[exact: add_stack_cwf|exact: add_stack_gwf|exact: add_stack_nwf].
   move=> y /Nbw; rewrite whites_add_stack.
   rewrite ![[disjoint successors _ & _]]disjoint_sym.
-   by apply/disjoint_trans/subsetDl.
-move=> [e1_wf e1_gwf Nbw1 black_sccs1] sube1 whites1 m_min.
+  by apply/disjoint_trans/subsetDl.
+move=> [e1_wf e1_cwf e1_gwf Nbw1 black_sccs1] sube1 whites1 m_min.
 have [//|s s_def sb] := subenv_stackP _ sube1.
 set s2 := rcons s x.
 have e1_uniq := @wf_uniq _ e1_wf.
@@ -747,28 +743,14 @@ have xe_uniq : uniq (x :: stack e).
 have x_stack : x \in stack e1 by rewrite s_def mem_cat mem_head orbT.
 have x_grays : x \in grays e1.
    by rewrite (subenv_grays sube1) grays_add_stack ?setU11.
-have rkx : rank x (x :: stack e) = rank x (stack e1).
-  by rewrite s_def rank_catl ?mem_head.
 have sx_subscc : is_subscc [set y in rcons s x].
   apply: (@is_subscc1 x); first by rewrite inE mem_rcons mem_head.
   move=> y; rewrite !inE mem_rcons in_cons => /predU1P [->//|y_s]; split.
     apply: (@wf_grays_to_stack e1) => //; first by rewrite s_def mem_cat y_s.
-    rewrite -rkx s_def rank_catr //=; last first.
-       by rewrite -(@uniq_catLR _ _ s) ?mem_cat ?y_s // -?s_def //.
-    rewrite rankE mem_head (leq_trans (index_size _ _)) //.
-    by rewrite size_rev leq_addr.
+    admit.
   have [] := @wf_stack_to_grays _ e1_gwf y; first by rewrite s_def mem_cat y_s.
   move=> z [z_gray rank_z] /connect_trans; apply.
-  rewrite (@wf_grays_to_stack e1) // s_def.
-  have := z_gray; rewrite graysE !(inE, s_def) mem_cat.
-  case: (boolP (z \in s)) => [/(subsetP sb)->//|_ /= /andP [_ z_xe]].
-  rewrite !rank_catl ?mem_head //.
-  move: z_xe; rewrite in_cons.
-  have [->//|neq_zx /= z_s] := altP eqP.
-  rewrite ltnW // rank_le_head //.
-  rewrite -(@uniq_catLR _ _ (rcons s x)) ?mem_rcons ?mem_head //.
-    by rewrite cat_rcons -s_def wf_uniq.
-  by rewrite mem_cat mem_rcons mem_head.
+  by rewrite (@wf_grays_to_stack e1) //; rewrite (subenv_gray_le sube1).
 have wreachex : wreach e x = x |: \bigcup_(y in [set y in successors x])
                           wreach (add_stack x e) y.
   rewrite /wreach whites_add_stack.
@@ -786,34 +768,50 @@ have wreachex : wreach e x = x |: \bigcup_(y in [set y in successors x])
   exists p => //; elim: p => [|z p ihp] //= in y {xy} neq_xy eyp xNp *.
   move: eyp xNp; rewrite in_cons -andbA => /and3P[yw yz ezp] /norP[neq_yz xNp].
   by rewrite !inE eq_sym neq_xy yw yz /= ihp.
-have m2_min : minn m m1 = \min_(y in wreach e x) @inord #|V| (rank y (stack e1)).
-  by rewrite wreachex bigmin_setU big_set1 //= /m rkx ord_rank // m_min.
+have m2_min : minn m m1 = \min_(y in wreach e x) @inord infty (num e1 y).
+  rewrite wreachex bigmin_setU big_set1 //= /m -m_min; congr (minn _ _).
+  rewrite (subenv_num sube1) ?mem_head//= ffunE/= eqxx.
+  by rewrite inordK// ltnS sn_small.
 have succ_whiteF z : z \in successors x -> z \in whites e1 = false.
   move=> z_successor; apply/negbTE.
   rewrite whites1 whites_add_stack !inE !negb_and !negbK.
   by rewrite (appP bigcupP idP) //; exists z; rewrite !inE.
 case: ltnP => [m1_small|m1_big] //=.
   rewrite (minn_idPr _) 1?ltnW// in m2_min.
-  have [x1 rank_x1 x_to_x1] : exists2 x1,
-    rank x1 (stack e1) = m1 & gconnect x x1.
+  have [x1 num_x1 x_to_x1] : exists2 x1, num e1 x1 = m1 & gconnect x x1.
       have [] := @eq_bigmin_cond _ _ (pred_of_set (wreach e x))
-                          (fun y => @inord #|V| (rank y (stack e1))).
+                          (fun y => @inord infty (num e1 y)).
         by apply/card_gt0P; exists x; rewrite mem_wreach.
       move=> y; rewrite !inE=> xy /(congr1 val)/=.
-      rewrite -m2_min ord_rank // => m1_eq; exists y => //.
+      rewrite -m2_min ord_num // => m1_eq; exists y => //.
       by apply: connect_sub xy => u v /= /andP [_]; apply: connect1.
-  have [x' [rank_x' x'_gray x_to_x' ]] : exists x',
-    [/\ rank x' (stack e1) < rank x (stack e1), x' \in grays e1 & gconnect x x'].
-    move: m1_small; rewrite -{}rank_x1 => rank_x1.
+  have [x' [num_x' x'_gray x_to_x' ]] : exists x',
+    [/\ num e1 x' < num e1 x, x' \in grays e1 & gconnect x x'].
+    (* move: m1_small; rewrite -{}num_x1 => num_x1. *)
     have x1_stack : x1 \in stack e1.
-      by rewrite -rank_lt ?(leq_trans rank_x1) // rank_le.
-    have [z [z_gray rank_z y_to_z]] := wf_stack_to_grays e1_gwf x1_stack.
+      rewrite num_stackP// num_x1 (leq_trans m1_small) ?andbT.
+        rewrite m2_min (_ : 1 = @inord infty 1); last by admit.
+        apply/bigmin_geqP => i; rewrite !inordK//=; last by admit.
+        rewrite lt0n wf_num0//.
+        rewrite wreachex !inE => /predU1P[->|].
+          by case: color4P x_stack. (* TODO: add this to ssrdone *)
+        by rewrite whites1 inE => ->.
+      by apply: leq_trans (subenv_sn sube1); rewrite leqW.
+    have [z [z_gray num_z y_to_z]] := wf_stack_to_grays e1_gwf x1_stack.
     exists z; split=> //; rewrite 2?inE ?z_gray ?andbT.
-    - by rewrite (leq_ltn_trans rank_z) // (leq_trans rank_x1) /m ?rkx.
+    - rewrite (leq_ltn_trans num_z)// num_x1 (leq_trans m1_small)// /m.
+      by rewrite (subenv_num sube1) ?mem_head //= ffunE/= eqxx. (* lemma *)
     - by rewrite (connect_trans x_to_x1).
-  have neq_x'x : x' != x by apply: contraTneq rank_x' => ->; rewrite -ltnNge.
+  have neq_x'x : x' != x by apply: contraTneq num_x' => ->; rewrite -ltnNge.
   split=> //.
-  - split=> //; first exact: add_blacks_ewf.
+  - split=> //; first exact: add_blacks_cwf.
+    + split => //.
+      * move=> y /=.
+        by rewrite whites_add_blacks wf_num0// subND1//; case: color4P x_grays.
+      * by move=> y /=; rewrite wf_num_infty.
+      * by move=> y /= /wf_num_lt; apply.
+      * by rewrite /= grays_add_blacks wf_sn// setUCA setUA setD1K.
+      * by move=> y z /= y_stack z_stack; rewrite wf_num_stack.
     + split => //.
         move=> y z /=; rewrite grays_add_blacks => y_gray z_stack.
         apply: wf_grays_to_stack => //; apply: subsetP y_gray.
@@ -844,20 +842,26 @@ case: ltnP => [m1_small|m1_big] //=.
         by rewrite (wf_grays_to_stack e1_gwf) // ltnW.
       have /scc_sub := x'_scc.
       rewrite !inE (negPf neq_x'x) /=.
-      by case: colorP x'_gray.
-  - apply/and4P; split => //=.
+      by case: color4P x'_gray.
+  - apply/and5P; split => //=.
     + rewrite grays_add_blacks (subenv_grays sube1) grays_add_stack ?setU1K //.
       by rewrite whites_graysF.
     + by rewrite (subset_trans (subenv_blacks sube1)) // subsetUr.
     + by rewrite -[sccs e]/(sccs (add_stack x e)) subenv_sccs.
+    + apply/forall_inP => y y_stack; apply/eqP.
+      rewrite (subenv_num sube1)/= ?in_cons ?y_stack ?orbT// ffunE/=.
+      by rewrite ifN//; apply: contraTneq xe_uniq => <- /=; rewrite y_stack.
     + apply/'exists_eqP/uniq_ex_drop; rewrite // s_def /=.
       by exists (rcons s x); rewrite cat_rcons.
   - rewrite whites_add_blacks big_set1 wreachex whites1 whites_add_stack.
     by rewrite !setDDl setUA setUAC setUid.
   - by rewrite m2_min; congr val; apply: eq_bigl=> y; rewrite /= big_set1.
-move: m2_min; rewrite (minn_idPl _) // /m rkx => rkx_min.
-have rkx_le y : y \in wreach e x -> rank y (stack e1) >= rank x (stack e1).
-  by move=> xy; rewrite rkx_min -ord_rank // geq_bigmin_cond.
+(* post conditions *)
+move: m2_min; rewrite (minn_idPl _) // => sn_min.
+have numx_le y : y \in wreach e x -> num e1 y >= num e1 x.
+  move=> xy; rewrite (@leq_trans m) //; last first.
+    by rewrite sn_min -ord_num// geq_bigmin_cond.
+  by rewrite (subenv_num sube1) ?mem_head//= ffunE/= eqxx. (*TODO: lemma*)
 have scc_max : scc_of x \subset [set y in s2].
   apply/subsetP=> y; rewrite inE=> y_sccx; apply: contraTT isT => yNs2.
   have xy : gconnect x y by have := y_sccx; rewrite mem_scc /= => /andP[].
@@ -869,7 +873,7 @@ have scc_max : scc_of x \subset [set y in s2].
   have xx' : gconnect x x'.
     by apply: connect_sub xx's2 => u v /= /andP[_]; apply: connect1.
   have /or3P[] : [|| y' \in whites e1, y' \in cover (sccs e1)
-                   | y' \in stack e1] by case: colorP.
+                   | y' \in stack e1] by case: color4P.
   - move: x'_s2; rewrite mem_rcons in_cons => /predU1P [eq_x'x|x_s].
       by rewrite succ_whiteF -?eq_x'x.
     have /(_ x') := Nbw1; rewrite (subsetP sb) => // /(_ isT).
@@ -880,7 +884,7 @@ have scc_max : scc_of x \subset [set y in s2].
     have : x \in scc_of y'.
       have:= y_sccx; rewrite !mem_scc /= andbC => /andP[yx _].
       by rewrite (connect_trans y'y) //= (connect_trans xx') //= connect1.
-    by move=> /(subsetP scc'_black); case: colorP x_grays.
+    by move=> /(subsetP scc'_black); case: color4P x_grays.
   - rewrite s_def -cat_rcons mem_cat (negPf y'Ns2) /= => y'_stack.
     have xNstack: x \notin stack e.
       rewrite -(@uniq_catLR _ x s2) ?mem_cat ?x_s2 //.
@@ -891,14 +895,15 @@ have scc_max : scc_of x \subset [set y in s2].
     have s2_whites: {subset s2 <= whites e}.
       move=> z z_s2; have: z \notin cover (sccs e).
         apply/negP=> /(subsetP (subset_cover (subenv_sccs sube1))).
-        suff: z \in stack e1 by case: colorP.
+        suff: z \in stack e1 by case: color4P.
         by rewrite s_def -cat_rcons mem_cat z_s2.
-      wlog: / z \in stack e by case: colorP; do ?[exact|move=>?].
+      wlog: / z \in stack e by case: color4P; do ?[exact|move=>?].
       have us2e : uniq (s2 ++ stack e) by rewrite cat_rcons -s_def.
       by rewrite (uniq_catRL us2e) ?mem_cat ?z_s2.
-    suff /rkx_le : y' \in wreach e x.
-      rewrite s_def !rank_catl ?mem_head ?in_cons ?y'_stack ?orbT //=.
-      by rewrite leqNgt rank_le_head.
+    suff /numx_le : y' \in wreach e x.
+      rewrite !(subenv_num sube1) ?mem_head//?in_cons ?y'_stack ?orbT//=.
+      rewrite !ffunE/= eqxx (negPf neq_y'x) leqNgt wf_num_lt//.
+      by rewrite wf_num_infty//; case: color4P y'_stack.
     rewrite !inE (@connect_trans _ _ x') //; last first.
        by rewrite connect1 /= ?s2_whites.
     apply: connect_sub xx's2 => u v /= /andP[/s2_whites uw uv].
@@ -917,9 +922,35 @@ have drop_s : drop (index x (stack e1)).+1 (stack e1) = stack e.
 split=> //.
 - split=> //.
   + by apply: add_sccs_wf=> //; rewrite take_s //.
-  + split=> //; rewrite ?grays_add_sccs ?stack_add_sccs ?take_s ?drop_s// ?g1Nx.
-      exact: wf_grays_to_stack.
-      exact: wf_stack_to_grays.
+  + split=> //=. (* TODO: generalize *)
+    * move=> y; rewrite whites_add_sccs// ?take_s//.
+      rewrite set_infty_eq0 ?wf_num0//= => z; rewrite mem_rcons in_cons wf_num0//.
+      by move=> /predU1P[->|/(subsetP sb)]; case: color4P x_stack.
+    * move=> y; rewrite !take_s.
+      rewrite /cover big_setU1/= -/(cover _).
+        by rewrite set_infty_eq_infty wf_num_infty// !inE.
+      suff: ~~ ([set y0 in rcons s x] \subset cover (sccs e1)).
+        apply: contra => sx_in.
+        by rewrite /cover (big_setD1 _ sx_in) /= subsetUl.
+      apply: contraTN isT => /subsetP /(_ x); rewrite inE mem_rcons in_cons eqxx/=.
+      by case: color4P x_grays => //= ??; apply.
+    * move=> y /=; rewrite !take_s set_infty_eq_infty/= negb_or => /andP[ysx nNinfty].
+      by rewrite set_infty_id ?ysx// wf_num_lt.
+    * by rewrite grays_add_sccs// ?take_s// setUCA setUA setD1K // wf_sn.
+    * rewrite drop_s take_s// => z t z_stack t_stack.
+      rewrite !set_infty_id/=; last 2 first.
+        - admit.
+        - admit.
+      rewrite !(subenv_num sube1) ?ffunE/=;
+        do ?by rewrite in_cons ?t_stack ?z_stack orbT.
+      rewrite !ifN ?wf_num_stack//.
+      - admit.
+      - admit.
+  + split=> //=; rewrite ?grays_add_sccs ?stack_add_sccs ?take_s ?drop_s// ?g1Nx.
+      (* exact: wf_grays_to_stack. *)
+      (* exact: wf_stack_to_grays. *)
+      admit.
+      admit.
   + move=> y; rewrite !inE whites_add_sccs ?take_s //.
     move=> /predU1P [->|/Nbw1//]; apply/pred0P=> z //=.
     by have [/succ_whiteF->|] := boolP (z \in successors x).
@@ -945,26 +976,37 @@ split=> //.
       by move=> _; rewrite -(def_scc _ x_scc) // (def_scc s2_gsccs) ?eqxx.
     rewrite -subDset (setDidPl _); first by move->; rewrite orbT.
     by rewrite disjoint_sym (@eq_disjoint1 _ x) // => y; rewrite !inE.
-- rewrite /subenv grays_add_sccs ?take_s ?sb ?g1Nx ?eqxx /= ?drop_s //=.
+- rewrite /= /subenv grays_add_sccs ?take_s ?sb ?g1Nx ?eqxx /= ?drop_s //=.
   rewrite (subset_trans (subenv_blacks sube1)) ?subsetUr //=.
   rewrite (subset_trans (subenv_sccs sube1)) ?subsetUr //=.
+  apply/andP; split.
+    by rewrite take_s; admit.
   by apply/'exists_eqP; exists ord0; rewrite drop0.
 - rewrite whites_add_sccs ?take_s ?sb //.
   by rewrite whites1 whites_add_stack big_set1 wreachex setDDl.
-- rewrite big_set1 /= drop_s; apply/eqP; rewrite eqn_leq leq_ord andbT.
-  rewrite -[#|V|]/(val ord_max); apply/bigmin_geqP => y /= /rkx_le.
-  apply: contraTT; rewrite -!ltnNge ord_rank// rank_lt // => y_stack.
-  rewrite !s_def !rank_catl ?mem_head ?in_cons ?y_stack ?orbT //=.
-  by rewrite rank_le_head //; case: colorP x_white.
-Qed.
+- rewrite big_set1 /= take_s; apply/eqP; rewrite eqn_leq leq_ord andbT.
+  rewrite [X in X <= _](_ : infty = @inord infty infty); last admit.
+  apply/bigmin_geqP => y /= /numx_le.
+  apply: contraTT; rewrite -!ltnNge ?inordK//; last admit.
+  rewrite set_infty_id; last admit.
+  rewrite [num _ x](subenv_num sube1) ?mem_head//= ffunE/= eqxx.
+  admit.
+
+(* rewrite wf_num_lt. *)
+
+(*  ord_num// rank_lt // => y_stack. *)
+(*   rewrite !s_def !rank_catl ?mem_head ?in_cons ?y_stack ?orbT //=. *)
+(*   by rewrite rank_le_head //; case: color4P x_white. *)
+(* Qed. *)
+Admitted.
 
 Theorem tarjan_rec_terminates n (roots : {set V}) e :
   n >= #|whites e| * #|V|.+1 + #|roots| ->
-  dfs'_correct (tarjan_rec n) roots e.
+  dfs_correct (tarjan_rec n) roots e.
 Proof.
 move=> n_ge; wlog ->: e n roots {n_ge} / roots = set0 => [noroot|]; last first.
-  have := @dfs'_is_correct (dfs1 (tarjan_rec 0)) (tarjan_rec 0) set0 e.
-  rewrite /tarjan_rec /dfs'_correct /dfs' /=.
+  have := @dfs_is_correct (dfs1 (tarjan_rec 0)) (tarjan_rec 0) set0 e.
+  rewrite /tarjan_rec /dfs_correct /dfs /=.
   case: n=> [|n /=]; case: pickP => [x|_/=]; rewrite ?inE //;
   by apply => ?; rewrite inE.
 have [V0|VN0] := posnP #|V|.
@@ -973,8 +1015,8 @@ have [V0|VN0] := posnP #|V|.
 elim: n => [|n IHn] in roots e n_ge *.
   move: n_ge; rewrite leqn0 addn_eq0 cards_eq0.
   by move=> /andP [_ /eqP/noroot]; apply.
-move=> pre; rewrite /dfs'_correct /=.
-apply: dfs'_is_correct => //= x x_root.
+move=> pre; rewrite /dfs_correct /=.
+apply: dfs_is_correct => //= x x_root.
   move=> x_white; apply: dfs1_is_correct => //; apply: IHn.
   rewrite whites_add_stack cardsDS ?sub1set // cards1 subn1.
   rewrite -ltnS (leq_trans _ n_ge) //.
@@ -988,16 +1030,20 @@ by rewrite ltn_add2l [X in _ < X](cardsD1 x) x_root.
 Qed.
 
 Lemma tarjan_rec_is_correct :
-  tarjan_rec N setT e0 = (infty, Env setT [::] gsccs).
+  tarjan_rec N setT e0 = (infty, Env setT [::] gsccs infty [ffun _ => infty]).
 Proof.
-have := @tarjan_rec_terminates N setT e0; rewrite /dfs'_correct.
+have := @tarjan_rec_terminates N setT e0; rewrite /dfs_correct.
 case: tarjan_rec => [m e] [].
 - by rewrite ?leq_add ?leq_mul ?max_card.
 - do ![split=> //; rewrite /= ?cover0 ?grays0 ?set0D ?setU0 //];
     do ?by[do [move=> ?|move/setP=> ?]; rewrite ?grays0 inE].
+  + by move=> x; rewrite ffunE whitesE grays0 !inE eqxx.
+  + by move=> x; rewrite ffunE inE eq_sym.
+  + by move=> x; rewrite ffunE.
+  + by rewrite cards0.
   apply/setP=> y; rewrite !inE /= subset0 andbC; case: eqP => //= ->.
   by have /and3P [_ _ /negPf->]:= gsccs_partition.
-move=> [[stack_wf _ _] _ _] sccse /subenv_grays grayse.
+move=> [[stack_wf _ _ e_nwf] _ _] sccse /subenv_grays grayse.
 rewrite (eqP _ : \bigcup_(x in _) _ = setT) ?setDT => [whe ->|]; last first.
   rewrite -subTset; apply/subsetP=> y _; apply/bigcupP.
   by exists y; rewrite ?mem_wreach.
@@ -1010,8 +1056,15 @@ have {sccse}sccse: sccs e = gsccs.
 have stacke : stack e = [::].
   have := stack_wf; rewrite sccse cover_gsccs setCT.
   by case: stack => // x s /(_ x); rewrite !inE eqxx.
-congr (_, _); last by case: (e) blackse sccse stacke => //= *; congr Env.
-by rewrite big1=> // x _; apply/val_inj; rewrite stacke /= ord_rank ?rank_infty.
+have sne : sn e = infty.
+  by rewrite wf_sn// grayse blackse grays0 set0U cardsT.
+have nume : num e = [ffun _ => infty].
+  apply/ffunP => x; rewrite ffunE; apply/eqP; rewrite wf_num_infty//.
+  by rewrite sccse cover_gsccs.
+congr (_, _); last first.
+  by case: (e) blackse sccse stacke sne nume => //= *; congr Env.
+rewrite big1 // => x _; apply/val_inj; rewrite /= ord_num//.
+by apply/eqP; rewrite wf_num_infty // sccse cover_gsccs.
 Qed.
 
 Theorem tarjan_correct : tarjan = gsccs.
